\chapter{Semantics}\label{app:semantics}
\subsection*{Arithmetic}
The semantics of statements and declarations both depend on the semantics of arithmetic expressions.
Arithmetic expressions may contain variables.

\subsubsection{Addition}
\begin{equation}
	\frac { { e }_{ v },st\vdash { a }_{ 1 }{ \rightarrow  }_{ A }{ v }_{ 1 }\quad { e }_{ v },st\vdash { a }_{ 2 }{ \rightarrow  }_{ A }{ v }_{ 2 } }{ { e }_{ v },st\vdash { a }_{ 1 }+{ a }_{ 2 }{ \rightarrow  }_{ A }{ v } } , v = { v }_{ 1 }+{ v }_{ 2 }
\end{equation}


\subsubsection{Subtraction}
\begin{equation}
	\frac { { e }_{ v },st\vdash { a }_{ 1 }{ \rightarrow  }_{ A }{ v }_{ 1 }\quad { e }_{ v },st\vdash { a }_{ 2 }{ \rightarrow  }_{ A }{ v }_{ 2 } }{ { e }_{ v },st\vdash { a }_{ 1 }-{ a }_{ 2 }{ \rightarrow  }_{ A }{ v } } ,\quad v={ v }_{ 1 }-{ v }_{ 2 }
\end{equation}


\subsubsection{Multiplication}
\begin{equation}
	\frac { { e }_{ v },st\vdash { a }_{ 1 }{ \rightarrow  }_{ A }{ v }_{ 1 }\quad { e }_{ v },st\vdash { a }_{ 2 }{ \rightarrow  }_{ A }{ v }_{ 2 } }{ { e }_{ v },st\vdash { a }_{ 1 }\ast { a }_{ 2 }{ \rightarrow  }_{ A }{ v } } ,\quad v={ v }_{ 1 }\ast { v }_{ 2 }
\end{equation}


\subsubsection{Boolean $\top$}
\begin{equation}
	\frac { { e }_{ v },st\vdash { a }_{ 1 }{ \rightarrow  }_{ A }{ v }_{ 1 }\quad { e }_{ v },st\vdash { a }_{ 2 }{ \rightarrow  }_{ A }{ v }_{ 2 } }{ { e }_{ v },st\vdash { a }_{ 1 }={ a }_{ 2 }{ \rightarrow  }true } ,{ v }_{ 1 }={ v }_{ 2 }\rightarrow true
\end{equation}


\subsubsection{Boolean $\bot$}
\begin{equation}
	\frac { { e }_{ v },st\vdash { a }_{ 1 }{ \rightarrow  }_{ A }{ v }_{ 1 }\quad { e }_{ v },st\vdash { a }_{ 2 }{ \rightarrow  }_{ A }{ v }_{ 2 } }{ { e }_{ v },st\vdash { a }_{ 1 }!={ a }_{ 2 }{ \rightarrow  }false } ,{ v }_{ 1 }={ v }_{ 2 }\rightarrow false
\end{equation}


\subsubsection{Parentheses}
\begin{equation}
	\frac { { e }_{ v },st\vdash { a }_{ 1 }{ \rightarrow  }_{ A }{ v } }{ { e }_{ v },st\vdash { (a }_{ 1 }){ \rightarrow  }_{ A }{ v } }
\end{equation}


\subsubsection{Variables}
\begin{equation}
	{ e }_{ v },st\vdash n{ \rightarrow  }_{ a }v, { e }_{ v }(x)=\iota\quad and\quad st(\iota )=v
\end{equation}


\subsection*{Declaring Variables}
Any non-empty variable declaration will modify the variable environment since the new variables will be bound to the new location.
A variable declaration will also modify the store, since the new location will be initialised to contain the initial values of the new variables.
The transition relation describing variable declarations defines a big-step semantic, since the allocation of new address space for newly declared variables is an invisible operation.

\subsubsection{Transition}
\begin{equation}
<{ D }_{ v },{ e }_{ v },st>{ \rightarrow  }_{ Dv }<{ e }_{ v }^{ ` },{ st }^{ ` }>
\end{equation}


\subsubsection{Empty Variables}
\begin{equation}
	<\varepsilon,{ e }_{ v },st>{ \rightarrow  }_{ DV }<{ e }_{ v },st>
\end{equation}


\subsubsection{Variable declaration}
\begin{equation}
	\frac { <{ D }_{ v },{ e }_{ v }^{ `` },st[\iota \mapsto v]>{ \rightarrow  }_{ Dv }<{ e }_{ v }^{ ` },{ st }^{ ` }> }{ <var\quad x:=a;Dv,{ e }_{ v }st>{ \rightarrow  }_{ Dv }<{ e }_{ v }^{ ` },{ st }^{ ` }> } 
\end{equation}
\begin{align*}
	where\quad &{ e }_{ v },st\vdash a{ \rightarrow  }_{ A }v \\
	&\iota {= e }_{ v }(next) \\
	&{ e }_{ v }^{ `` }={ e }_{ v }[x\mapsto \iota ][next\mapsto new \iota ]
\end{align*}

\begin{equation}
	{ D }_{ v }::=var x:=a; { D }_{ v } | \varepsilon
\end{equation}


\subsection*{Statements}
The effect of a statement is that the store may change, since a statement may modify the values of variables involved through assignments.
A statement should not modify the variable environment.
We define a BS-semantic for statements (except procedure calls)
\subsubsection{Transitions}
\begin{equation}
	{ e }_{ v },{ e }_{ p }\vdash <S,st>\rightarrow { st }^{ ` }
\end{equation}


\subsubsection{Transition system}
\begin{equation}
	{((Stm\ast  Sto)\cup Sto \rightarrow Sto) }
\end{equation}


\subsubsection{Assignment}
\begin{align*}
	&{ e }_{ v }\vdash <x=a,st>\rightarrow st[\iota \mapsto v]\\
	where\quad &{ e }_{ v },st\vdash a{ \rightarrow  }_{ A }v\quad and\quad  { e }_{ v }(x)=\iota 
\end{align*}


\subsubsection{Skip}
\begin{equation}
	{ e }_{ v }\vdash <skip,st>\rightarrow st
\end{equation}


\subsubsection{Compare}
\begin{equation}
	\frac { { e }_{ v }\vdash <{ s }_{ 1 },st>\rightarrow { st }^{ `` }\quad { e }_{ v }\vdash <{ S }_{ 2 },{ st }^{ `` }>\rightarrow { st }^{ ` } }{ { e }_{ v },\vdash <{ s }_{ 1 };{ s }_{ 2 },st>\rightarrow { st }^{ ` } } 
\end{equation}


\subsubsection{If $\top$}
\begin{equation}
	\frac { { e }_{ v }\vdash <{ s }_{ 1 },st>\rightarrow { st }^{ ` } }{ { e }_{ v }\vdash <if\quad b\quad then\quad { S }_{ 1 }\quad else{ \quad S }_{ 2 }>\rightarrow { st }^{ ` } } st\vdash b{ \rightarrow  }_{ B }\top 
\end{equation}

\subsubsection{If $\bot$}
\begin{equation}
	\frac { { e }_{ v }\vdash <{ s }_{ 1 },st>\rightarrow { st }^{ ` } }{ { e }_{ v }\vdash <if\quad b\quad then\quad { S }_{ 1 }\quad else{ \quad S }_{ 2 }>\rightarrow { st }^{ ` } } st\vdash b{ \rightarrow  }_{ B }\bot 
\end{equation}


\subsubsection{While $\top$}
\begin{align*}
	&\frac { { e }_{ v }\vdash <{ S }_{ 1 },st>\rightarrow { st }^{ `` }\quad { e }_{ v }\vdash <while\quad b\quad do\quad S,st>\rightarrow { st }^{ ` } }{ { e }_{ v }\vdash <while\quad b\quad do\quad S,st>\rightarrow { st }^{ ` } }\\
	&if\quad { e }_{ v },st\vdash b{ \rightarrow  }_{ B }\top 
\end{align*}


\subsubsection{While $\bot$}
\begin{align*}
	&{ e }_{ v }\vdash <while\quad b\quad do\quad S,\quad st>\rightarrow st\\
	&if\quad { e }_{ v },st\vdash b{ \rightarrow  }_{ B }\bot
\end{align*}

\subsubsection{Blocks}
\begin{align*}
&<D,{ e }_{ v },st>{ \rightarrow  }_{ DV }<{ e }_{ v }^{ ` },{ st }^{ `` }>\\
&{ e }_{ v }^{ ` }\vdash <{ D }_{ p }>{ \rightarrow  }_{ Dv }<{ e }_{ v }^{ ` },{ st }^{ `` }>\\
&\frac { { e }_{ v }^{ ` }\vdash <S,{ st }^{ `` }>\rightarrow { st }^{ ` } }{ { e }_{ v }\vdash <begin\quad { D }_{ v }\quad { D }_{ p },st>\rightarrow { st }^{ ` } } 
\end{align*}

\subsubsection{Return}
\begin{equation}
	\frac { { e }_{ v }\vdash <{ s },st>{ \rightarrow  }_{ s }v,{ st }^{ ` } }{ { e }_{ v }\vdash <(s)|return;,{ e }_{ v },st>{ \rightarrow  }_{ A }v,{ e }_{ v }{ st }^{ ` } } 
\end{equation}


\subsection*{Matrices and vectors}
\subsubsection{Matrix declaration}
\begin{equation}
	\frac { { e }_{ v },st\vdash j{ \rightarrow  }_{ A }{ v }_{ 1 }\quad { e }_{ v },st\vdash k{ \rightarrow  }_{ A }{ v }_{ 2 } }{ { M }^{ 1 }\quad =\quad martix<int|float|bool>[{ v }_{ 1 },{ v }_{ 2 }]\rightarrow { st }^{ ` },{ e }_{ v } } ,{ M }^{ 1 }[{ v }_{ 1 },{ v }_{ 2 }]=\begin{bmatrix} { { 0 }_{ 1,1 } } & \dots  & { 0 }_{ { 1,{ v }_{ 2 } } } \\ \vdots  & \ddots  &  \\ { 0 }_{ { v }_{ 1 },1 } &  & { 0 }_{ { v }_{ 1 },{ v }_{ 2 } } \end{bmatrix}
\end{equation}

\subsubsection{Addition}
\begin{equation}
	\frac { { e }_{ v },st\vdash { M }^{ 1 }{ \rightarrow  }_{ A }{ v }_{ 1 }\quad { e }_{ v },st\vdash { M }^{ 2 }{ \rightarrow  }_{ A }{ v }_{ 2 } }{ { e }_{ v },st\vdash { M }^{ 1 }+{ M }^{ 2 }{ \rightarrow  }_{ A }{ v } } ,\begin{matrix} { v }_{ 1 }=matrix<>[j,k] \\ { v }_{ 2 }=matrix<>[j,k] \\ v=\begin{bmatrix} { { m }_{ 1,1 }^{ 1 } } +{ { m }_{ 1,1 }^{ 2 } } & { { m }_{ 2,1 }^{ 1 } } + { { m }_{ 2,1 }^{ 2 } } & \dots  & { m }_{ 1,k }^{ 1 }+{ { m }_{ 1,k }^{ 2} } \\
{ { m }_{ 2,1 }^{ 1 } } + { { m }_{ 2,1 }^{ 2 } } &  { { m }_{ 2,2 }^{ 1 } } +{ { m }_{ 2,2 }^{ 2 } } & \dots & { { m }_{ 2,k }^{ 1 } } + { { m }_{ 2,k }^{ 2 } }
\\ \vdots  & \vdots & \ddots  & \vdots \\
 { m }_{ j,1 }^{ 1 } +{ { m }_{ j,1 }^{ 2 } } & { { m }_{ j,2 }^{ 1 } } +{ { m }_{ j,2 }^{ 2 } }  & \dots & { m }_{ j,k }^{ 1 }+{ { m }_{ j,k }^{ 2 } } \end{bmatrix}

 \end{matrix}
\end{equation}


\subsubsection{Subtraction}
\begin{equation}
	\frac { { e }_{ v },st\vdash { M }^{ 1 }{ \rightarrow  }_{ A }{ v }_{ 1 }\quad { e }_{ v },st\vdash { M }^{ 2 }{ \rightarrow  }_{ A }{ v }_{ 2 } }{ { e }_{ v },st\vdash { M }^{ 1 }-{ M }^{ 2 }{ \rightarrow  }_{ A }{ v } } ,\begin{matrix} { v }_{ 1 }=matrix<>[j,k] \\ { v }_{ 2 }=matrix<>[j,k] \\ v=\begin{bmatrix} { { m }_{ 1,1 }^{ 1 } } - { { m }_{ 1,1 }^{ 2 } } & { { m }_{ 2,1 }^{ 1 } } - { { m }_{ 2,1 }^{ 2 } } & \dots  & { m }_{ 1,k }^{ 1 } - { { m }_{ 1,k }^{ 2} } \\
{ { m }_{ 2,1 }^{ 1 } } - { { m }_{ 2,1 }^{ 2 } } &  { { m }_{ 2,2 }^{ 1 } } - { { m }_{ 2,2 }^{ 2 } } & \dots & { { m }_{ 2,k }^{ 1 } }  - { { m }_{ 2,k }^{ 2 } }
\\ \vdots  & \vdots & \ddots  & \vdots \\
 { m }_{ j,1 }^{ 1 } - { { m }_{ j,1 }^{ 2 } } & { { m }_{ j,2 }^{ 1 } } - { { m }_{ j,2 }^{ 2 } }  & \dots & { m }_{ j,k }^{ 1 } - { { m }_{ j,k }^{ 2 } } \end{bmatrix} \end{matrix}
\end{equation}


\subsubsection{Matrix product}
\begin{minipage}{1.0\textwidth}
\begin{equation}
\begin{aligned}
	\frac { { e }_{ v },st\vdash { M }^{ 1 }{ \rightarrow  }_{ A }{ v }_{ 1 }\quad { e }_{ v },st\vdash { M }^{ 2 }{ \rightarrow  }_{ A }{ v }_{ 2 } }{ { e }_{ v },st\vdash { M }^{ 1 }*{ M }^{ 2 }{ \rightarrow  }_{ A }{ v } } ,\begin{matrix} { v }_{ 1 }=matrix<>[j,k] \\ { v }_{ 2 }=matrix<>[k,l] \\
	 v=\begin{bmatrix} { { m }_{ 1,1 }^{ 3 } } & { { m }_{ 2,1 }^{ 3 } } & \dots  & { m }_{ 1,l }^{ 3 }\\
{ { m }_{ 2,1 }^{ 3 } } &   +{ { m }_{ 2,2 }^{ 3 } } & \dots & { { m }_{ 2,l }^{ 3 } }
\\ \vdots  & \vdots & \ddots  & \vdots  \\
 { m }_{ j,1 }^{ 3 }& { { m }_{ j,2 }^{ 3 } } & \dots & { m }_{ j,l }^{ 3 } \end{bmatrix} where
\\ \end{matrix}
\end{aligned}
\end{equation}
\begin{equation*}
\begin{aligned}
{ { m }_{ 1,1 }^{ 3 } }  = { { m }_{ 1,1 }^{ 1 } } *{ { m }_{ 1,1 }^{ 2 } }+ { { m }_{ 1,2 }^{ 1 } } *{ { m }_{ 2,1 }^{ 2 } }+\dots+ { { m }_{ 1,k }^{ 1 } } *{ { m }_{ k,1 }^{ 2 } }\\
{ { m }_{ 1,2 }^{ 3 } }  = { { m }_{ 1,1 }^{ 1 } } *{ { m }_{ 1,2 }^{ 2 } }+ { { m }_{ 1,2 }^{ 1 } } *{ { m }_{ 2,2 }^{ 2 } }+\dots+ { { m }_{ 1,k }^{ 1 } } *{ { m }_{ k,2 }^{ 2 } }\\
{ { m }_{ 1,k }^{ 3 } }  = { { m }_{ 1,1 }^{ 1 } } *{ { m }_{ 1,k }^{ 2 } }+ { { m }_{ 1,2 }^{ 1 } } *{ { m }_{ 2,k }^{ 2 } }+\dots+ { { m }_{ 1,j }^{ 1 } } *{ { m }_{ j,l }^{ 2 } }\\
{ { m }_{ 2,1 }^{ 3 } }  = { { m }_{ 2,1 }^{ 1 } } *{ { m }_{ 1,1 }^{ 2 } }+ { { m }_{ 2,2 }^{ 1 } } *{ { m }_{ 2,1 }^{ 2 } }+\dots+ { { m }_{ 2,k }^{ 1 } } *{ { m }_{ k,1 }^{ 2 } }\\
{ { m }_{ 2,2 }^{ 3 } }  = { { m }_{ 2,1 }^{ 1 } } *{ { m }_{ 1,l }^{ 2 } }+ { { m }_{ 2,2 }^{ 1 } } *{ { m }_{ 2,2 }^{ 2 } }+\dots+ { { m }_{ 2,k }^{ 1 } } *{ { m }_{ k,2 }^{ 2 } }\\
{ { m }_{ 2,l }^{ 3 } }  = { { m }_{ 2,1 }^{ 1 } } *{ { m }_{ 1,l }^{ 2 } }+ { { m }_{ 2,2 }^{ 1 } } *{ { m }_{ 2,l }^{ 2 } }+\dots+ { { m }_{ 2,k }^{ 1 } } *{ { m }_{ k,l }^{ 2 } }\\
{ { m }_{ j,1 }^{ 3 } }  = { { m }_{ j,1 }^{ 1 } } *{ { m }_{ 1,1 }^{ 2 } }+ { { m }_{ j,2 }^{ 1 } } *{ { m }_{ 2,1 }^{ 2 } }+\dots+ { { m }_{ j,k }^{ 1 } } *{ { m }_{ k,1 }^{ 2 } }\\
{ { m }_{ j,2 }^{ 3 } }  = { { m }_{ j,1 }^{ 1 } } *{ { m }_{ 1,2 }^{ 2 } }+ { { m }_{ j,2 }^{ 1 } } *{ { m }_{ 2,2 }^{ 2 } }+\dots+ { { m }_{ j,k }^{ 1 } } *{ { m }_{ k,2 }^{ 2 } }\\
{ { m }_{ j,l }^{ 3 } }  = { { m }_{ j,1 }^{ 1 } } *{ { m }_{ 1,l }^{ 2 } }+ { { m }_{ j,2 }^{ 1 } } *{ { m }_{ 2,l }^{ 2 } }+\dots+ { { m }_{ j,k }^{ 1 } } *{ { m }_{ k,l }^{ 2 } }
\end{aligned}
\end{equation*}
\end{minipage}

\subsubsection{Scalar product}
\begin{equation}
	\frac { { e }_{ v },st\vdash { M }^{ 1 }{ \rightarrow  }_{ A }{ v }_{ 1 }\quad { e }_{ v },st\vdash { a }_{ 1 }{ \rightarrow  }_{ A }{ v }_{ 2 } }{ { e }_{ v },st\vdash { M }^{ 1 }\ast { a }_{ 1 }{ \rightarrow  }_{ A }{ v } } ,\begin{matrix} { v }_{ 1 }=matrix<>[j,k] \\ { v }_{ 2 }={ a }_{ 1 } \\ v=\begin{bmatrix} { { a }_{ 1 }*m }_{ 1,1 }^{ 1 } & { { a }_{ 1 }*m }_{ 1,2 }^{ 1 } & \dots  & { { a }_{ 1 }*m }_{ 1,k }^{ 1 } \\
 { { a }_{ 1 }*m }_{ 2,1 }^{ 1 } & { { a }_{ 1 }*m }_{ 2,2 }^{ 1 } & \dots  & { { a }_{ 1 }*m }_{ 2,k }^{ 1 }  \\ \vdots & \vdots & \ddots & \vdots \\ { { a }_{ 1 }*m }_{ j,1 }^{ 1 } & { { a }_{ 1 }*m }_{ j,2 }^{ 1 } & \dots & { { a }_{ 1 }*m }_{ j,k }^{ 1 } \end{bmatrix} \end{matrix}
\end{equation}

\subsubsection{Transposed Matrix}
\begin{equation}
	\frac { { e }_{ v },st\vdash { m }_{ 1 }{ \rightarrow  }_{ A }{ v }_{ 1 }\quad  }{ { e }_{ v },st\vdash { m }_{ 1 }\wedge { \rightarrow  }_{ A }{ v } } ,\begin{matrix} { v }_{ 1 }=matrix<>[j,k] \\ { v }={ v }_{ 1 }\wedge[k,j] =\begin{bmatrix} { { m }_{ 1,1 }^{ 1 } } & { { m }_{ 2,1 }^{ 1 } } & \dots  & { m }_{ j,1 }^{ 1 } \\
{ { m }_{ 1,2 }^{ 1 } }  &  { { m }_{ 2,2 }^{ 1 } } & \dots & { m }_{ j,2 }^{ 1 }
\\ \vdots  & \vdots & \ddots  & \vdots \\
 { m }_{ 1,k }^{ 1 } & { m }_{ 2,k }^{ 1 } & \dots & { m }_{ k,j }^{ 1 } \end{bmatrix} \end{matrix}
\end{equation}

\subsubsection{Mulindex Matrix}
\begin{equation}
	\frac { { e }_{ v },st\vdash { M }^{ 1 }{ \rightarrow  }_{ A }{ v }_{ 1 }\quad { e }_{ v },st\vdash { M }^{ 2 }{ \rightarrow  }_{ A }{ v }_{ 2 } }{ { e }_{ v },st\vdash { M }^{ 1 }\ast { M }^{ 2 }{ \rightarrow  }_{ A }{ v } } ,\begin{matrix} { v }_{ 1 }=matrix<>[j,k] \\ { { v }_{ 2 } }=matrix<>[j,k] \\ v=\begin{bmatrix} { { m }_{ 1,1 }^{ 1 } } * { { m }_{ 1,1 }^{ 2 } } & { { m }_{ 2,1 }^{ 1 } } * { { m }_{ 2,1 }^{ 2 } } & \dots  & { m }_{ 1,k }^{ 1 } * { { m }_{ 1,k }^{ 2} } \\
{ { m }_{ 2,1 }^{ 1 } } * { { m }_{ 2,1 }^{ 2 } } &  { { m }_{ 2,2 }^{ 1 } } * { { m }_{ 2,2 }^{ 2 } } & \dots & { { m }_{ 2,k }^{ 1 } }  * { { m }_{ 2,k }^{ 2 } }
\\ \vdots  & \vdots & \ddots  & \vdots \\
 { m }_{ j,1 }^{ 1 } * { { m }_{ j,1 }^{ 2 } } & { { m }_{ j,2 }^{ 1 } } * { { m }_{ j,2 }^{ 2 } }  & \dots & { m }_{ j,k }^{ 1 } * { { m }_{ j,k }^{ 2 } } \end{bmatrix} \end{matrix}
\end{equation}

\subsubsection{Vector Dot Product}
\begin{equation}
	\frac { { e }_{ v },st\vdash { { vec } }^{ 1 }{ \rightarrow  }_{ A }{ v }^{ 1 }\quad { e }_{ v },st\vdash { { { vec } }^{ 2 } }{ \rightarrow  }_{ A }{ v }_{ 2 } }{ { e }_{ v },st\vdash { { vec } }^{ 1 }\ast { { vec } }^{ 2 }{ \rightarrow  }_{ A }{ v } } ,\begin{matrix} { v }_{ 1 }=vector<>[{ n }] \\ { v }_{ 2 }=vector<>[{ n }] \\ v={ vec }_{ 1 }^{ 1 }*{ vec }_{ 1 }^{ 2 }+\dots +{ vec }_{ n }^{ 1 }*{ vec }_{ n }^{ 2 } \\  \end{matrix}
\end{equation}